CPO.v
@@ -1,0 +1,191 @@
+From Stdlib Require Import Utf8.
+From Paco Require Import paco.
+
+Set Primitive Projections.
+
+Variant StreamF {T Stream} :=
+| snil
+| scons (hd : T) (tl : Stream)
+| stau (tl : Stream)
+.
+
+Arguments StreamF : clear implicits.
+
+CoInductive Stream {T} := mkStream { obs_st : StreamF T Stream }.
+
+Arguments Stream : clear implicits.
+
+Notation Snil := {| obs_st := snil |}.
+Notation Scons hd tl := {| obs_st := scons hd tl |}.
+Notation Stau tl := {| obs_st := stau tl |}.
+
+(* define approximation order *)
+Inductive le_StreamF {T le_Stream} (s s' : Stream T) : Prop :=
+| le_snil
+  (NIL : obs_st s = snil)
+| le_scons_scons hd tl tl'
+  (CONS : obs_st s = scons hd tl)
+  (CONS' : obs_st s' = scons hd tl')
+  (LE : le_Stream tl tl')
+| le_stauL tl
+  (TAU : obs_st s = stau tl)
+  (LE : le_StreamF tl s')
+| le_stauR tl'
+  (TAU' : obs_st s' = stau tl')
+  (LE : le_StreamF s tl')
+| le_stauB tl tl'
+  (TAU : obs_st s = stau tl)
+  (TAU' : obs_st s' = stau tl')
+  (LE : le_Stream tl tl')
+.
+
+Arguments le_StreamF {_} _ _ _.
+
+Lemma le_StreamF_monotone T : monotone2 (@le_StreamF T).
+Proof.
+  repeat intro. induction IN.
+  - econstructor 1; eauto.
+  - econstructor 2; eauto.
+  - econstructor 3; eauto.
+  - econstructor 4; eauto.
+  - econstructor 5; eauto.
+Qed.
+
+Hint Resolve le_StreamF_monotone : paco.
+
+Definition le_Stream {T} := paco2 (@le_StreamF T) bot2.
+
+Lemma le_Stream_refl {T} : ∀ s, le_Stream (T := T) s s.
+Proof.
+  pcofix CIH.
+  intros. pfold. destruct (obs_st s) eqn:EQ.
+  - econstructor 1; eauto.
+  - econstructor 2; eauto.
+  - econstructor 5; eauto.
+Qed.
+
+Lemma inv_tauL {T} :
+  ∀ s s' (LE : le_Stream (T := T) s s') tl (TAUL : obs_st s = stau tl),
+    le_Stream tl s'.
+Proof.
+  do 3 intro. punfold LE. induction LE.
+  - intros. congruence.
+  - intros. congruence.
+  - intros. rewrite TAUL in *. inversion TAU; subst; clear TAU.
+    pfold; auto.
+  - intros. pfold. econstructor 4; eauto.
+    specialize (IHLE _ TAUL). punfold IHLE.
+  - intros. rewrite TAUL in *. inversion TAU; subst; clear TAU.
+    pclearbot. pfold. econstructor 4; eauto. punfold LE.
+Qed.
+
+Lemma inv_tauR {T} :
+  ∀ s s' (LE : le_Stream (T := T) s s') tl' (TAUR : obs_st s' = stau tl'),
+    le_Stream s tl'.
+Proof.
+  do 3 intro. punfold LE. induction LE.
+  - intros. pfold. econstructor 1; eauto.
+  - intros. congruence.
+  - intros. pfold. econstructor 3; eauto.
+    specialize (IHLE _ TAUR). punfold IHLE.
+  - intros. rewrite TAUR in *. inversion TAU'; subst; clear TAU'.
+    pfold; auto.
+  - intros. rewrite TAUR in *. inversion TAU'; subst; clear TAU'.
+    pclearbot. pfold. econstructor 3; eauto. punfold LE.
+Qed.
+
+Lemma inv_nilR {T} :
+  ∀ s s' s''
+    (LE' : le_Stream (T := T) s' s'')
+    (LE : le_Stream s s')
+    (OBS : obs_st s'' = snil),
+    le_Stream s s''.
+Proof.
+  pcofix CIH.
+  do 4 intro. revert s. punfold LE'. induction LE'.
+  - intros. pfold. clear CIH. revert s' OBS. rename s0 into s''.
+    punfold LE. induction LE.
+    + intros. econstructor 1; eauto.
+    + congruence.
+    + specialize (IHLE NIL). intros. econstructor 3; eauto.
+    + congruence.
+    + congruence.
+  - intros. congruence.
+  - intros. eapply IHLE'; eauto. eapply inv_tauR; eauto.
+  - intros. congruence.
+  - intros. congruence.
+Qed.
+
+Lemma inv_nil_all {T} :
+  ∀ s s'
+    (LE : le_Stream (T := T) s s')
+    (OBS : obs_st s' = snil)
+    s'',
+    le_Stream s s''.
+Proof.
+  pcofix CIH.
+  do 3 intro. punfold LE. induction LE.
+  - intros. pfold. econstructor 1; eauto.
+  - intros; congruence.
+  - intros. pfold. econstructor 3; eauto. specialize (IHLE OBS s''). punfold IHLE.
+  - intros. congruence.
+  - intros; congruence.
+Qed.
+
+Lemma le_Stream_trans {T} :
+  ∀ s s' s'',
+    le_Stream (T := T) s s' → le_Stream s' s'' → le_Stream s s''.
+Proof.
+  pcofix CIH.
+  do 3 intro. intros LE LE'. revert s'' LE'.
+  punfold LE.
+  induction LE.
+  - intros. pfold. econstructor 1; eauto.
+  - intros. pclearbot. punfold LE'. induction LE'; rewrite CONS' in *.
+    + congruence.
+    + inversion CONS0; subst; clear CONS0.
+      pclearbot. pfold. econstructor 2; eauto.
+    + congruence.
+    + pfold. econstructor 4; eauto.
+      specialize (IHLE' eq_refl).
+      punfold IHLE'.
+    + congruence.
+  - intros. specialize (IHLE _ LE'). pfold. econstructor 3; eauto.
+    punfold IHLE.
+  - intros. eapply IHLE. eapply inv_tauL; eauto.
+  - intros. pclearbot.
+    assert (le_Stream s s') as LE'' by (pfold; econstructor 5; eauto).
+    destruct (obs_st s'') as [|hd'' tl''|tl''] eqn:OBS.
+    { specialize (inv_nilR s s' s'' LE' LE'' OBS).
+      intros. eapply paco2_mon; eauto. destruct 1. }
+    punfold LE'. revert hd'' tl'' OBS.
+    clear tl tl' TAU TAU' LE.
+    rename LE'' into LE.
+    revert s LE.
+    induction LE'; intros.
+    + specialize (inv_nil_all _ _ LE NIL s').
+      intros. eapply paco2_mon; eauto. destruct 1.
+    + rewrite OBS in *. inversion CONS'; subst; clear CONS'.
+      pclearbot. punfold LE0. revert LE0.
+      induction 1.
+      * pfold. econstructor 1; eauto.
+      * rewrite CONS in *. inversion CONS'; subst; clear CONS'.
+        pclearbot. pfold. econstructor 2; eauto.
+      * pfold. econstructor 3; eauto. specialize (IHLE0 CONS). punfold IHLE0.
+      * rewrite CONS in *. congruence.
+      * rewrite CONS in *. congruence.
+    + eapply IHLE'; eauto. clear IHLE' hd'' tl'' OBS LE' s'.
+      revert tl TAU. punfold LE. induction LE; intros; try rewrite TAU in *.
+      * pfold. econstructor 1; eauto.
+      * congruence.
+      * pfold. econstructor 3; eauto.
+        specialize (IHLE _ TAU0). punfold IHLE.
+      * inversion TAU'; subst; clear TAU'. pfold. auto.
+      * rewrite TAU0 in *. inversion TAU'; subst; clear TAU'.
+        pclearbot. pfold. econstructor 3; eauto. punfold LE.
+    + congruence.
+    + congruence.
+    + pfold. econstructor 5; eauto. right. eapply CIH; eauto.
+      eapply inv_tauL; eauto. eapply inv_tauR; eauto.
+Qed.
+
